verified/entry.i.dfy
@@ -1,0 +1,167 @@
+include "entry.s.dfy"
+
+lemma MICommute(s1:SysState, s2:SysState, s3:SysState, p:PageNr)
+    requires validSysState(s1) && validSysState(s2) && validSysState(s3) &&
+        s1.d == s2.d == s3.d && validL1PTPage(s1.d, p) &&
+        (validPageDbImpliesWellFormed(s1.d); !hasStoppedAddrspace(s1.d, p))
+    requires WSMemInvariantExceptAddrspaceAtPage(s1, s2, p) &&
+        WSMemInvariantExceptAddrspaceAtPage(s2, s3, p)
+    ensures WSMemInvariantExceptAddrspaceAtPage(s1, s3, p)
+{
+}
+
+predicate {:opaque} validResume_premium(s:SysState,s':SysState,dispPage:PageNr)
+    requires validSysState(s)
+    ensures validResume_premium(s, s', dispPage) == validResume(s, s', dispPage)
+    ensures (smc_resume(s.d, dispPage).1 == KEV_ERR_SUCCESS()
+             && validResume(s, s', dispPage)) ==> 
+        validSysState(s')
+        && bankedRegsPreservedForMonitor(s, s')
+        && (var p := l1pOfDispatcher(s.d, dispPage);
+            validL1PTPage(s.d, p)
+            && (validPageDbImpliesWellFormed(s.d); !hasStoppedAddrspace(s.d, p))
+            && WSMemInvariantExceptAddrspaceAtPage(s, s', p))
+{
+    if(smc_resume(s.d, dispPage).1 == KEV_ERR_SUCCESS() && validResume(s, s', 
+        dispPage)) then
+        valResImpliesMInv(s, s', dispPage);
+        valResImpliesBRPres(s, s', dispPage);
+        validResume(s, s', dispPage)
+    else
+        validResume(s, s', dispPage)
+    
+}
+
+lemma valResImpliesBRPres(s:SysState,s':SysState,dispPage:PageNr)
+    requires validSysState(s)
+    requires smc_resume(s.d, dispPage).1 == KEV_ERR_SUCCESS()
+        && validResume(s, s', dispPage)
+    ensures bankedRegsPreservedForMonitor(s, s')
+{
+    
+    forall( s2, s3, s4 | validEntryTransitionResume(s,s2,dispPage) 
+        && userspaceExecution(s2, s3)
+        && exception(s3, s4)
+        && monitorReturn(s4, s') )
+        ensures bankedRegsPreservedForMonitor(s, s')
+    {
+        assert bankedRegsPreservedForMonitor(s, s2);
+        assert bankedRegsPreservedForMonitor(s2, s3);
+        assert bankedRegsPreservedForMonitor(s3, s4);
+        assert bankedRegsPreservedForMonitor(s4, s');
+    }
+}
+
+lemma valResImpliesMInv(s:SysState,s':SysState,dispPage:PageNr)
+    requires validSysState(s)
+    requires smc_resume(s.d, dispPage).1 == KEV_ERR_SUCCESS()
+                && validResume(s, s', dispPage)
+    ensures
+        validSysState(s) && validSysState(s') && s'.d == s.d
+    ensures
+        var p := l1pOfDispatcher(s.d, dispPage);
+        validL1PTPage(s.d, p)
+        && (validPageDbImpliesWellFormed(s.d); !hasStoppedAddrspace(s.d, p))
+        && WSMemInvariantExceptAddrspaceAtPage(s, s', p)
+{   
+    forall( s2, s3, s4 | validEntryTransitionResume(s,s2,dispPage) 
+        && userspaceExecution(s2, s3)
+        && exception(s3, s4)
+        && monitorReturn(s4, s') )
+        ensures WSMemInvariantExceptAddrspaceAtPage(s, s', 
+            l1pOfDispatcher(s.d, dispPage))
+    {
+        var p := l1pOfDispatcher(s.d, dispPage);
+        assert WSMemInvariantExceptAddrspaceAtPage(s,  s2, p);
+        assert s2.hw.conf.ttbr0 == p;
+        assert WSMemInvariantExceptAddrspaceAtPage(s2, s3, p);
+        assert s3.hw.conf.ttbr0 == s2.hw.conf.ttbr0;
+        assert s3.hw.conf.ttbr0 == p;
+        assert WSMemInvariantExceptAddrspaceAtPage(s3, s4, p);
+        assert s4.hw.conf.ttbr0 == p;
+        assert WSMemInvariantExceptAddrspaceAtPage(s4, s', p);
+        MICommute(s, s2, s3, p);
+        MICommute(s, s3, s4, p);
+        MICommute(s, s4, s', p);
+    }
+}
+
+lemma valEnterImpliesBRPres(s:SysState,s':SysState,dispPage:PageNr,
+    a1:int,a2:int,a3:int)
+    requires isUInt32(a1) && isUInt32(a2) && isUInt32(a3) && validSysState(s)
+    requires smc_enter(s.d, dispPage,a1,a2,a3).1 == KEV_ERR_SUCCESS()
+        && validEnter(s, s', dispPage,a1,a2,a3)
+    ensures bankedRegsPreservedForMonitor(s, s')
+{
+    
+    forall( s2, s3, s4 | validEntryTransitionEnter(s,s2,dispPage,a1,a2,a3) 
+        && userspaceExecution(s2, s3)
+        && exception(s3, s4)
+        && monitorReturn(s4, s') )
+        ensures bankedRegsPreservedForMonitor(s, s')
+    {
+        assert bankedRegsPreservedForMonitor(s, s2);
+        assert bankedRegsPreservedForMonitor(s2, s3);
+        assert bankedRegsPreservedForMonitor(s3, s4);
+        assert bankedRegsPreservedForMonitor(s4, s');
+    }
+}
+
+lemma valEnterImpliesMInv(s:SysState,s':SysState,dispPage:PageNr,
+    a1:int,a2:int,a3:int)
+    requires isUInt32(a1) && isUInt32(a2) && isUInt32(a3) && validSysState(s)
+    requires smc_enter(s.d, dispPage,a1,a2,a3).1 == KEV_ERR_SUCCESS()
+                && validEnter(s, s', dispPage,a1,a2,a3)
+    ensures
+        validSysState(s) && validSysState(s') && s'.d == s.d
+    ensures
+        var p := l1pOfDispatcher(s.d, dispPage);
+        validL1PTPage(s.d, p)
+        && (validPageDbImpliesWellFormed(s.d); !hasStoppedAddrspace(s.d, p))
+        && WSMemInvariantExceptAddrspaceAtPage(s, s', p)
+{   
+    forall( s2, s3, s4 | validEntryTransitionEnter(s,s2,dispPage,a1,a2,a3) 
+        && userspaceExecution(s2, s3)
+        && exception(s3, s4)
+        && monitorReturn(s4, s') )
+        ensures WSMemInvariantExceptAddrspaceAtPage(s, s', 
+            l1pOfDispatcher(s.d, dispPage))
+    {
+        var p := l1pOfDispatcher(s.d, dispPage);
+        assert WSMemInvariantExceptAddrspaceAtPage(s,  s2, p);
+        assert s2.hw.conf.ttbr0 == p;
+        assert WSMemInvariantExceptAddrspaceAtPage(s2, s3, p);
+        assert s3.hw.conf.ttbr0 == s2.hw.conf.ttbr0;
+        assert s3.hw.conf.ttbr0 == p;
+        assert WSMemInvariantExceptAddrspaceAtPage(s3, s4, p);
+        assert s4.hw.conf.ttbr0 == p;
+        assert WSMemInvariantExceptAddrspaceAtPage(s4, s', p);
+        MICommute(s, s2, s3, p);
+        MICommute(s, s3, s4, p);
+        MICommute(s, s4, s', p);
+    }
+}
+
+predicate {:opaque} validEnter_premium(s:SysState,s':SysState,dispPage:PageNr,
+    a1:int,a2:int,a3:int)
+    requires isUInt32(a1) && isUInt32(a2) && isUInt32(a3) && validSysState(s)
+    ensures validEnter_premium(s, s', dispPage,a1,a2,a3)
+        == validEnter(s, s', dispPage,a1,a2,a3)
+    ensures (smc_enter(s.d, dispPage,a1,a2,a3).1 == KEV_ERR_SUCCESS()
+             && validEnter(s, s', dispPage,a1,a2,a3)) ==> 
+        validSysState(s')
+        && bankedRegsPreservedForMonitor(s, s')
+        && (var p := l1pOfDispatcher(s.d, dispPage);
+            validL1PTPage(s.d, p)
+            && (validPageDbImpliesWellFormed(s.d); !hasStoppedAddrspace(s.d, p))
+            && WSMemInvariantExceptAddrspaceAtPage(s, s', p))
+{
+    if(smc_enter(s.d, dispPage,a1,a2,a3).1 == KEV_ERR_SUCCESS() && validEnter(s, s', 
+        dispPage,a1,a2,a3)) then
+        valEnterImpliesMInv(s, s', dispPage,a1,a2,a3);
+        valEnterImpliesBRPres(s, s', dispPage,a1,a2,a3);
+        validEnter(s, s', dispPage,a1,a2,a3)
+    else
+        validEnter(s, s', dispPage,a1,a2,a3)
+    
+}
